lib/Base/KeyType.s.dfy
@@ -3,8 +3,21 @@ include "NativeTypes.s.dfy"
 module {:extern} KeyType {
   import NativeTypes
 
-  function method MaxLen() : NativeTypes.uint64 { 20 }
-  type Key = s : seq<NativeTypes.byte> | |s| <= 20
+  function method {:extern} MaxLen() : NativeTypes.uint64
+  //type Key = s : seq<NativeTypes.byte> | |s| <= 20
+  type Key(!new,==)
+
+  function method {:extern} seq_to_key(s: seq<NativeTypes.byte>) : Key
+  requires |s| <= 20
+
+  function method {:extern} key_to_seq(k: Key) : seq<NativeTypes.byte>
+
+  function method {:extern} KeyLenUint64(key: Key): NativeTypes.uint64
+
+  function method {:extern} key_cmp(a: Key, b: Key): NativeTypes.int32
+
+  method {:extern "KeyType_Compile", "CopyKeyIntoArray"} CopyKeyIntoArray(src:Key, dst:array<NativeTypes.byte>, dstIndex:NativeTypes.uint64)
+
 }
 
 module {:extern} ValueType {
